examples/lambda/barendregt/head_reductionScript.sml
@@ -1,3 +1,7 @@
+(*---------------------------------------------------------------------------*
+ * Head Reductions of Lambda Terms                                           *
+ *---------------------------------------------------------------------------*)
+
 open HolKernel Parse boolLib bossLib BasicProvers;
 
 open boolSimps relationTheory pred_setTheory listTheory finite_mapTheory
@@ -5,13 +9,12 @@ open boolSimps relationTheory pred_setTheory listTheory finite_mapTheory
      hurdUtils;
 
 open termTheory appFOLDLTheory chap2Theory chap3Theory nomsetTheory binderLib
-     horeductionTheory term_posnsTheory finite_developmentsTheory;
+     horeductionTheory term_posnsTheory finite_developmentsTheory
+     basic_swapTheory;
 
 val _ = new_theory "head_reduction"
 
 val _ = ParseExtras.temp_loose_equality()
-
-fun Store_thm(trip as (n,t,tac)) = store_thm trip before export_rewrites [n]
 
 Inductive hreduce1 :
 [~BETA:]
@@ -145,12 +148,56 @@ Proof
  >> fs [hreduce1_rules]
 QED
 
-Theorem hreduce1_LAMl :
-    !vs M1 M2. M1 -h-> M2 ==> LAMl vs M1 -h-> LAMl vs M2
+Theorem hreduce_BETA_extended :
+    !l vs t. LAMl vs t @* MAP VAR vs @* MAP VAR l -h->* t @* MAP VAR l
 Proof
-    Induct_on ‘vs’ >> rw []
- >> MATCH_MP_TAC hreduce1_LAM
- >> FIRST_X_ASSUM MATCH_MP_TAC >> art []
+    Q.X_GEN_TAC ‘l’
+ >> Induct_on ‘vs’ >- rw []
+ >> rw [Once RTC_CASES1]
+ >> DISJ2_TAC
+ >> qabbrev_tac ‘M = LAMl vs t’
+ >> Q.EXISTS_TAC ‘[VAR h/h] M @* MAP VAR vs @* MAP VAR l’
+ >> reverse CONJ_TAC >- rw [Abbr ‘M’]
+ >> REWRITE_TAC [GSYM appstar_APPEND]
+ >> MATCH_MP_TAC hreduce1_rules_appstar
+ >> rw [hreduce1_BETA]
+QED
+
+(* |- !vs t. LAMl vs t @* MAP VAR vs -h->* t *)
+Theorem hreduce_BETA[simp] =
+        hreduce_BETA_extended |> Q.SPEC ‘[]’
+                              |> REWRITE_RULE [MAP, appstar_empty]
+
+Theorem hreduce1_LAMl[simp] :
+    !vs M1 M2. LAMl vs M1 -h-> LAMl vs M2 <=> M1 -h-> M2
+Proof
+    Induct_on ‘vs’
+ >> rw [Once hreduce1_rwts]
+QED
+
+Theorem hreduce_LAMl[simp] :
+    !vs M1 M2. LAMl vs M1 -h->* LAMl vs M2 <=> M1 -h->* M2
+Proof
+    rpt GEN_TAC
+ >> reverse EQ_TAC
+ >- (Q.ID_SPEC_TAC ‘M2’ \\
+     Q.ID_SPEC_TAC ‘M1’ \\
+     HO_MATCH_MP_TAC RTC_INDUCT >> rw [] \\
+     ONCE_REWRITE_TAC [RTC_CASES1] >> DISJ2_TAC \\
+     Q.EXISTS_TAC ‘LAMl vs M1'’ >> rw [])
+ >> Q.ID_SPEC_TAC ‘vs’
+ >> Induct_on ‘vs’ >> rw []
+ >> FIRST_X_ASSUM MATCH_MP_TAC
+ >> POP_ASSUM MP_TAC
+ >> Suff ‘!M2 M. M -h->* LAM h M2 ==> !M1. (M = LAM h M1) ==> M1 -h->* M2’
+ >- PROVE_TAC []
+ >> Q.X_GEN_TAC ‘M2’
+ >> HO_MATCH_MP_TAC RTC_ALT_INDUCT >> rw []
+ >> Q.PAT_X_ASSUM ‘LAM h M1 -h-> M'’ MP_TAC
+ >> rw [Once hreduce1_rwts]
+ >> rename1 ‘M1 -h-> M0’
+ >> ONCE_REWRITE_TAC [RTC_CASES1] >> DISJ2_TAC
+ >> Q.EXISTS_TAC ‘M0’ >> rw []
 QED
 
 Theorem hreduce1_abs :
@@ -313,7 +360,7 @@ Proof
        Q.PAT_X_ASSUM ‘h = v’ (fs o wrap) \\
       ‘FV M DELETE v = FV M’ by ASM_SET_TAC [] >> fs [] \\
        Q.PAT_X_ASSUM ‘!vs t. P’ (MP_TAC o (Q.SPECL [‘vs’, ‘t’])) >> rw [] \\
-       fs [FOLDR_APPEND] \\
+       fs [LAMl_APPEND] \\
        qexistsl_tac [‘v::vs1’, ‘vs2’, ‘N’] >> rw [],
        (* goal 2 (of 4) *)
        fs [tpm_eqr, tpm_LAMl] \\
@@ -612,10 +659,11 @@ val wh_is_abs = store_thm(
   ``∀M N. M -w-> N ⇒ ¬is_abs M``,
   HO_MATCH_MP_TAC weak_head_ind THEN SRW_TAC [][]);
 
-val wh_lam = Store_thm(
-  "wh_lam",
-  ``∀v M N. ¬(LAM v M -w-> N)``,
-  ONCE_REWRITE_TAC [weak_head_cases] THEN SRW_TAC [][]);
+Theorem wh_lam[simp] :
+    ∀v M N. ¬(LAM v M -w-> N)
+Proof
+  ONCE_REWRITE_TAC [weak_head_cases] THEN SRW_TAC [][]
+QED
 
 val wh_head = store_thm(
   "wh_head",
@@ -679,18 +727,19 @@ val bnf_whnf = store_thm(
   ``bnf M ⇒ whnf M``,
   METIS_TAC [hnf_whnf, bnf_hnf]);
 
-val whnf_thm = Store_thm(
-  "whnf_thm",
-  ``whnf (VAR s) ∧
+Theorem whnf_thm[simp] :
+   whnf (VAR s) ∧
     (whnf (M @@ N) ⇔ ¬is_abs M ∧ whnf M) ∧
-    whnf (LAM v M)``,
+    whnf (LAM v M)
+Proof
   REPEAT CONJ_TAC THEN SRW_TAC [][whnf_def, Once weak_head_cases] THEN
   EQ_TAC THEN SRW_TAC [][FORALL_AND_THM] THENL [
     Q.SPEC_THEN `M` FULL_STRUCT_CASES_TAC term_CASES THEN SRW_TAC [][] THEN
     METIS_TAC [],
     Q.SPEC_THEN `M` FULL_STRUCT_CASES_TAC term_CASES THEN
     FULL_SIMP_TAC (srw_ss()) []
-  ]);
+  ]
+QED
 
 val wh_weaken_cong = store_thm(
   "wh_weaken_cong",
@@ -766,12 +815,13 @@ val whstar_lameq = store_thm(
   ``M -w->* N ⇒ M == N``,
   METIS_TAC [betastar_lameq, whstar_betastar]);
 
-val whstar_abs = Store_thm(
-  "whstar_abs",
-  ``LAM v M -w->* N ⇔ (N = LAM v M)``,
+Theorem whstar_abs[simp] :
+    LAM v M -w->* N ⇔ (N = LAM v M)
+Proof
   SRW_TAC [][EQ_IMP_THM] THEN
   FULL_SIMP_TAC (srw_ss()) [Once relationTheory.RTC_CASES1,
-                            Once weak_head_cases]);
+                            Once weak_head_cases]
+QED
 
 (* ----------------------------------------------------------------------
     has_whnf
@@ -1544,7 +1594,7 @@ Proof
  >> rw [Once hnf_children_def]
 QED
 
-Theorem hnf_children_hnf :
+Theorem hnf_children_hnf[simp] :
     !y args. hnf_children (VAR y @* args) = args
 Proof
     rpt GEN_TAC
@@ -1859,6 +1909,277 @@ Proof
  >> ‘Ns = MAP SND pi’ by rw [Abbr ‘pi’, MAP_ZIP]
  >> simp []
  >> MATCH_MP_TAC hreduce_LAMl_appstar_lemma >> rw []
+QED
+
+val _ = hide "Y";
+
+(* NOTE: ‘permutator n’ contains n + 1 binding variables. Appending at most n
+   arbitrary terms, each head reduction step consumes just one of them,
+   eventually there should be one more fresh variable left, forming a hnf.
+
+   NOTE2: added one global excluded list X and more disjointness conclusions.
+ *)
+Theorem permutator_hreduce_thm :
+    !X n Ns. FINITE X /\ LENGTH Ns <= n ==>
+             ?xs y. permutator n @* Ns -h->*
+                    LAMl xs (LAM y (VAR y @* Ns @* MAP VAR xs)) /\
+                    ALL_DISTINCT (SNOC y xs) /\
+                    DISJOINT X (set (SNOC y xs)) /\
+                    !N. MEM N Ns ==> DISJOINT (FV N) (set (SNOC y xs))
+Proof
+    rw [permutator_def]
+ >> qabbrev_tac ‘Z = GENLIST n2s (n + 1)’
+ >> ‘ALL_DISTINCT Z /\ (LENGTH Z = n + 1)’
+       by (rw [Abbr ‘Z’, ALL_DISTINCT_GENLIST])
+ >> ‘Z <> []’ by rw [NOT_NIL_EQ_LENGTH_NOT_0]
+ >> qabbrev_tac ‘z = LAST Z’
+ >> ‘MEM z Z’ by rw [Abbr ‘z’, MEM_LAST_NOT_NIL]
+ >> qabbrev_tac ‘M = VAR z @* MAP VAR (FRONT Z)’
+ (* preparing for LAMl_ALPHA_ssub *)
+ >> qabbrev_tac
+     ‘Y = NEWS (n + 1) (X UNION set Z UNION (BIGUNION (IMAGE FV (set Ns))))’
+ >> Know ‘FINITE (X UNION set Z UNION (BIGUNION (IMAGE FV (set Ns))))’
+ >- (rw [] >> rw [FINITE_FV])
+ >> DISCH_TAC
+ >> Know ‘ALL_DISTINCT Y /\
+          DISJOINT (set Y) (X UNION set Z UNION (BIGUNION (IMAGE FV (set Ns)))) /\
+         (LENGTH Y = n + 1)’
+ >- (ASM_SIMP_TAC std_ss [NEWS_def, Abbr ‘Y’])
+ >> rw [] (* all disjointness are separated *)
+ (* applying LAMl_ALPHA_ssub *)
+ >> Know ‘LAMl Z M = LAMl Y ((FEMPTY |++ ZIP (Z,MAP VAR Y)) ' M)’
+ >- (MATCH_MP_TAC LAMl_ALPHA_ssub >> rw [DISJOINT_SYM] \\
+     Suff ‘FV M = set Z’ >- METIS_TAC [DISJOINT_SYM] \\
+     rw [Abbr ‘M’, FV_appstar] \\
+    ‘Z = SNOC (LAST Z) (FRONT Z)’ by PROVE_TAC [SNOC_LAST_FRONT] \\
+     POP_ORW \\
+     simp [LIST_TO_SET_SNOC] \\
+     rw [Once EXTENSION, MEM_MAP] \\
+     EQ_TAC >> rw [] >> fs [] \\
+     DISJ2_TAC \\
+     Q.EXISTS_TAC ‘FV (VAR x)’ >> rw [] \\
+     Q.EXISTS_TAC ‘VAR x’ >> rw [])
+ >> Rewr'
+ >> ‘Y <> []’ by rw [NOT_NIL_EQ_LENGTH_NOT_0]
+ >> REWRITE_TAC [GSYM fromPairs_def]
+ >> qabbrev_tac ‘fm = fromPairs Z (MAP VAR Y)’
+ >> ‘FDOM fm = set Z’ by rw [FDOM_fromPairs, Abbr ‘fm’]
+ >> qabbrev_tac ‘y = LAST Y’
+ >> ‘!t. LAMl Y t = LAMl (SNOC y (FRONT Y)) t’
+       by (ASM_SIMP_TAC std_ss [Abbr ‘y’, SNOC_LAST_FRONT]) >> POP_ORW
+ >> REWRITE_TAC [LAMl_SNOC]
+ >> Know ‘fm ' M = VAR y @* MAP VAR (FRONT Y)’
+ >- (simp [Abbr ‘M’, ssub_appstar] \\
+     Know ‘fm ' z = VAR y’
+     >- (rw [Abbr ‘fm’, Abbr ‘z’, LAST_EL] \\
+         Know ‘fromPairs Z (MAP VAR Y) ' (EL (PRE (n + 1)) Z) =
+               EL (PRE (n + 1)) (MAP VAR Y)’
+         >- (MATCH_MP_TAC fromPairs_FAPPLY_EL >> rw []) >> Rewr' \\
+         rw [EL_MAP, Abbr ‘y’, LAST_EL]) >> Rewr' \\
+     Suff ‘MAP ($' fm) (MAP VAR (FRONT Z)) = MAP VAR (FRONT Y)’ >- rw [] \\
+     rw [LIST_EQ_REWRITE, LENGTH_FRONT] \\
+    ‘PRE (n + 1) = n’ by rw [] >> POP_ASSUM (fs o wrap) \\
+     rename1 ‘i < n’ \\
+     simp [EL_MAP, LENGTH_FRONT] \\
+     Know ‘MEM (EL i (FRONT Z)) Z’
+     >- (rw [MEM_EL] \\
+         Q.EXISTS_TAC ‘i’ >> rw [] \\
+         MATCH_MP_TAC EL_FRONT >> rw [LENGTH_FRONT, NULL_EQ]) \\
+     rw [Abbr ‘fm’] \\
+     Know ‘EL i (FRONT Z) = EL i Z’
+     >- (MATCH_MP_TAC EL_FRONT >> rw [LENGTH_FRONT, NULL_EQ]) >> Rewr' \\
+     Know ‘EL i (FRONT Y) = EL i Y’
+     >- (MATCH_MP_TAC EL_FRONT >> rw [LENGTH_FRONT, NULL_EQ]) >> Rewr' \\
+     Know ‘fromPairs Z (MAP VAR Y) ' (EL i Z) = EL i (MAP VAR Y)’
+     >- (MATCH_MP_TAC fromPairs_FAPPLY_EL >> rw []) >> Rewr' \\
+     rw [EL_MAP])
+ >> Rewr'
+ (* stage work *)
+ >> qabbrev_tac ‘t = LAM y (VAR y @* MAP VAR (FRONT Y))’
+ >> qabbrev_tac ‘vs = FRONT Y’
+ >> ‘LENGTH vs = n’ by rw [LENGTH_FRONT, Abbr ‘vs’]
+ (* now break vs into two parts, the first part will match Ns's length *)
+ >> qabbrev_tac ‘k = LENGTH Ns’
+ >> qabbrev_tac ‘vs1 = TAKE k vs’
+ >> qabbrev_tac ‘vs2 = DROP k vs’
+ >> Know ‘ALL_DISTINCT vs’
+ >- (qunabbrev_tac ‘vs’ \\
+     MATCH_MP_TAC ALL_DISTINCT_FRONT >> art [])
+ >> DISCH_TAC
+ >> ‘vs = vs1 ++ vs2’ by rw [Abbr ‘vs1’, Abbr ‘vs2’, TAKE_DROP]
+ >> POP_ORW
+ >> REWRITE_TAC [LAMl_APPEND]
+ >> qabbrev_tac ‘t1 = LAMl vs2 t’
+ (* applying hreduce_LAMl_appstar *)
+ >> Know ‘LAMl vs1 t1 @* Ns -h->* (FEMPTY |++ ZIP (vs1,Ns)) ' t1’
+ >- (MATCH_MP_TAC hreduce_LAMl_appstar \\
+     CONJ_TAC >- (qunabbrev_tac ‘vs1’ \\
+                  MATCH_MP_TAC ALL_DISTINCT_TAKE >> art []) \\
+     CONJ_TAC >- (rw [Abbr ‘vs1’]) \\
+     rw [EVERY_MEM] \\
+     Know ‘DISJOINT (FV e) (set Y)’
+     >- (FIRST_X_ASSUM MATCH_MP_TAC >> Q.EXISTS_TAC ‘e’ >> art []) \\
+     Suff ‘(set vs1) SUBSET (set Y)’ >- PROVE_TAC [DISJOINT_SUBSET] \\
+     simp [SUBSET_DEF, Abbr ‘vs1’, Abbr ‘vs’] \\
+     METIS_TAC [MEM_TAKE, MEM_FRONT_NOT_NIL])
+ (* stage work *)
+ >> simp [GSYM fromPairs_def, Abbr ‘t1’]
+ >> ‘FDOM (fromPairs vs1 Ns) = set vs1’
+       by rw [Abbr ‘vs1’, Abbr ‘k’, FDOM_fromPairs]
+ (* applying LAMl_ssub to move ‘LAMl vs2’ out *)
+ >> Know ‘fromPairs vs1 Ns ' (LAMl vs2 t) = LAMl vs2 (fromPairs vs1 Ns ' t)’
+ >- (MATCH_MP_TAC LAMl_ssub >> rw []
+     >- (Q.PAT_X_ASSUM ‘ALL_DISTINCT vs’ MP_TAC \\
+        ‘vs = vs1 ++ vs2’ by rw [Abbr ‘vs1’, Abbr ‘vs2’, TAKE_DROP] \\
+         POP_ORW \\
+         rw [ALL_DISTINCT_APPEND, DISJOINT_ALT]) \\
+     rename1 ‘MEM v vs1’ \\
+     rfs [MEM_EL] >> rename1 ‘i < LENGTH vs1’ \\
+     Know ‘fromPairs vs1 Ns ' (EL i vs1) = EL i Ns’
+     >- (MATCH_MP_TAC fromPairs_FAPPLY_EL \\
+         Q.PAT_X_ASSUM ‘ALL_DISTINCT vs’ MP_TAC \\
+        ‘vs = vs1 ++ vs2’ by rw [Abbr ‘vs1’, Abbr ‘vs2’, TAKE_DROP] \\
+         POP_ORW \\
+         rw [ALL_DISTINCT_APPEND] \\
+         rw [Abbr ‘vs1’]) >> Rewr' \\
+     MATCH_MP_TAC DISJOINT_SUBSET \\
+     Q.EXISTS_TAC ‘set Y’ \\
+     reverse CONJ_TAC
+     >- (rw [SUBSET_DEF, Abbr ‘vs2’, Abbr ‘vs’, MEM_DROP, MEM_EL] \\
+         Q.PAT_X_ASSUM ‘LENGTH Y = LENGTH (FRONT Y) + 1’
+           (ONCE_REWRITE_TAC o wrap o SYM) \\
+         ASM_SIMP_TAC std_ss [REWRITE_RULE [NULL_EQ] EL_FRONT] \\
+         Q.EXISTS_TAC ‘k + m’ >> art [] \\
+         rfs [LENGTH_FRONT]) \\
+     FIRST_X_ASSUM MATCH_MP_TAC \\
+     Q.EXISTS_TAC ‘EL i Ns’ >> art [] \\
+     Q.EXISTS_TAC ‘i’ >> art [] \\
+     Suff ‘LENGTH Ns = LENGTH vs1’ >- rw [] \\
+     rw [Abbr ‘vs1’])
+ >> Rewr'
+ (* stage work *)
+ >> qunabbrev_tac ‘t’
+ >> qabbrev_tac ‘t = VAR y @* MAP VAR vs’
+ (* applying ssub_LAM to move ‘LAM y’ out of ssub *)
+ >> Know ‘fromPairs vs1 Ns ' (LAM y t) = LAM y (fromPairs vs1 Ns ' t)’
+ >- (MATCH_MP_TAC ssub_LAM >> simp [] \\
+     Q.PAT_X_ASSUM ‘ALL_DISTINCT Y’ MP_TAC \\
+     Know ‘SNOC y vs = Y’
+     >- (qunabbrevl_tac [‘y’, ‘vs’] \\
+         MATCH_MP_TAC SNOC_LAST_FRONT >> art []) \\
+     DISCH_THEN (ONCE_REWRITE_TAC o wrap o SYM) \\
+     rw [ALL_DISTINCT_SNOC]
+     >- (qunabbrev_tac ‘vs1’ >> PROVE_TAC [MEM_TAKE]) \\
+     rename1 ‘MEM v vs1’ >> POP_ASSUM MP_TAC >> rw [MEM_EL] \\
+     Know ‘fromPairs vs1 Ns ' (EL n vs1) = EL n Ns’
+     >- (MATCH_MP_TAC fromPairs_FAPPLY_EL \\
+         Q.PAT_X_ASSUM ‘ALL_DISTINCT vs’ MP_TAC \\
+        ‘vs = vs1 ++ vs2’ by rw [Abbr ‘vs1’, Abbr ‘vs2’, TAKE_DROP] \\
+         POP_ORW \\
+         rw [ALL_DISTINCT_APPEND] \\
+         rw [Abbr ‘vs1’]) >> Rewr' \\
+     Q.PAT_X_ASSUM ‘!s. _ ==> DISJOINT s (set Y)’
+       (MP_TAC o (Q.SPEC ‘FV (EL n (Ns :term list))’)) \\
+     Know ‘(?x. (FV (EL n Ns) = FV x) /\ MEM x Ns)’
+     >- (Q.EXISTS_TAC ‘EL n Ns’ >> rw [MEM_EL] \\
+         Q.EXISTS_TAC ‘n’ >> rw [Abbr ‘k’] \\
+         Suff ‘LENGTH Ns = LENGTH vs1’ >- rw [] \\
+         rw [Abbr ‘vs1’]) \\
+     Rewr \\
+     rw [DISJOINT_ALT'] \\
+     POP_ASSUM MATCH_MP_TAC \\
+     rw [Abbr ‘y’, MEM_LAST_NOT_NIL])
+ >> Rewr'
+ >> Know ‘~MEM y vs1’
+ >- (Q.PAT_X_ASSUM ‘ALL_DISTINCT Y’ MP_TAC \\
+     Know ‘SNOC y vs = Y’
+     >- (qunabbrevl_tac [‘y’, ‘vs’] \\
+         MATCH_MP_TAC SNOC_LAST_FRONT >> art []) \\
+     DISCH_THEN (ONCE_REWRITE_TAC o wrap o SYM) \\
+     rw [ALL_DISTINCT_SNOC] \\
+     qunabbrev_tac ‘vs1’ >> PROVE_TAC [MEM_TAKE])
+ >> DISCH_TAC
+ >> simp [Abbr ‘t’, ssub_appstar]
+ >> ‘vs = vs1 ++ vs2’ by rw [Abbr ‘vs1’, Abbr ‘vs2’, TAKE_DROP]
+ >> POP_ORW
+ >> REWRITE_TAC [MAP_APPEND]
+ >> Know ‘MAP ($' (fromPairs vs1 Ns)) (MAP VAR vs1) = Ns’
+ >- (rw [LIST_EQ_REWRITE] >- rw [Abbr ‘vs1’] \\
+     rename1 ‘i < LENGTH vs1’ \\
+     simp [EL_MAP] \\
+     Know ‘MEM (EL i vs1) vs1’
+     >- (rw [MEM_EL] >> Q.EXISTS_TAC ‘i’ >> art []) >> Rewr \\
+     MATCH_MP_TAC fromPairs_FAPPLY_EL >> rw []
+     >- (Q.PAT_X_ASSUM ‘ALL_DISTINCT vs’ MP_TAC \\
+        ‘vs = vs1 ++ vs2’ by rw [Abbr ‘vs1’, Abbr ‘vs2’, TAKE_DROP] \\
+         POP_ORW \\
+         rw [ALL_DISTINCT_APPEND, DISJOINT_ALT]) \\
+     rw [Abbr ‘vs1’])
+ >> Rewr'
+ >> Know ‘MAP ($' (fromPairs vs1 Ns)) (MAP VAR vs2) = MAP VAR vs2’
+ >- (rw [LIST_EQ_REWRITE] \\
+     rename1 ‘i < LENGTH vs2’ \\
+     rw [EL_MAP, MEM_EL] \\
+  (* NOTE: below we show conflicts in assumptions *)
+     Q.PAT_X_ASSUM ‘ALL_DISTINCT vs’ MP_TAC \\
+    ‘vs = vs1 ++ vs2’ by rw [Abbr ‘vs1’, Abbr ‘vs2’, TAKE_DROP] \\
+     POP_ORW \\
+     rw [ALL_DISTINCT_APPEND, DISJOINT_ALT] \\
+     METIS_TAC [MEM_EL])
+ >> Rewr'
+ (* final stage *)
+ >> REWRITE_TAC [appstar_APPEND]
+ >> DISCH_TAC
+ >> qexistsl_tac [‘vs2’, ‘y’] >> art []
+ (* extra goal: ALL_DISTINCT *)
+ >> CONJ_TAC
+ >- (reverse (rw [ALL_DISTINCT_SNOC])
+     >- (qunabbrev_tac ‘vs2’ \\
+         MATCH_MP_TAC ALL_DISTINCT_DROP >> art []) \\
+     Q.PAT_X_ASSUM ‘ALL_DISTINCT Y’ MP_TAC \\
+     Know ‘SNOC y vs = Y’
+     >- (qunabbrevl_tac [‘y’, ‘vs’] \\
+         MATCH_MP_TAC SNOC_LAST_FRONT >> art []) \\
+     DISCH_THEN (ONCE_REWRITE_TAC o wrap o SYM) \\
+     rw [ALL_DISTINCT_SNOC] \\
+     CCONTR_TAC >> fs [Abbr ‘vs2’] \\
+     PROVE_TAC [MEM_DROP_IMP])
+ (* extra goal: DISJOINT *)
+ >> CONJ_TAC
+ >- (reverse (rw [LIST_TO_SET_SNOC])
+     >- (Q.PAT_X_ASSUM ‘DISJOINT X (set Y)’ MP_TAC \\
+         rw [DISJOINT_ALT'] \\
+         POP_ASSUM MATCH_MP_TAC \\
+         rw [Abbr ‘y’, MEM_LAST_NOT_NIL]) \\
+     MATCH_MP_TAC DISJOINT_SUBSET \\
+     Q.EXISTS_TAC ‘set Y’ >> art [] \\
+     MATCH_MP_TAC SUBSET_TRANS \\
+     Q.EXISTS_TAC ‘set vs’ \\
+     reverse CONJ_TAC
+     >- (rw [SUBSET_DEF, Abbr ‘vs’] \\
+         MATCH_MP_TAC MEM_FRONT_NOT_NIL >> art []) \\
+     rw [SUBSET_DEF, Abbr ‘vs2’] \\
+     PROVE_TAC [MEM_DROP_IMP])
+ (* final stage *)
+ >> reverse (rw [LIST_TO_SET_SNOC])
+ >- (Suff ‘DISJOINT (FV N) (set Y)’
+     >- (rw [DISJOINT_ALT'] \\
+         POP_ASSUM MATCH_MP_TAC \\
+         rw [Abbr ‘y’, MEM_LAST_NOT_NIL]) \\
+     FIRST_X_ASSUM MATCH_MP_TAC \\
+     Q.EXISTS_TAC ‘N’ >> art [])
+ (* DISJOINT (FV N) (set vs2) *)
+ >> MATCH_MP_TAC DISJOINT_SUBSET
+ >> Q.EXISTS_TAC ‘set Y’
+ >> CONJ_TAC >- (FIRST_X_ASSUM MATCH_MP_TAC \\
+                 Q.EXISTS_TAC ‘N’ >> art [])
+ >> MATCH_MP_TAC SUBSET_TRANS
+ >> Q.EXISTS_TAC ‘set vs’
+ >> reverse CONJ_TAC
+ >- (rw [SUBSET_DEF, Abbr ‘vs’] \\
+     MATCH_MP_TAC MEM_FRONT_NOT_NIL >> art [])
+ >> rw [SUBSET_DEF, Abbr ‘vs2’]
+ >> PROVE_TAC [MEM_DROP_IMP]
 QED
 
 val _ = export_theory()
